Cleanned up perm_incl.v. Proved new ways of proving such permission inclusions.

perm_incl.v
@@ -2,43 +2,106 @@ From iris.algebra Require Import upred_big_op.
 From iris.program_logic Require Import thread_local.
 From lrust Require Export type perm.
 
-Section perm_incl.
+Import Perm.
+
+Section defs.
 
   Context `{heapG Σ, lifetimeG Σ, thread_localG Σ}.
 
+  (* Definitions *)
   Definition perm_incl (ρ1 ρ2 : perm) :=
     ∀ tid, ρ1 tid ={⊤}=> ρ2 tid.
 
-  Lemma perm_incl_top ρ : perm_incl ρ ⊤.
-  Proof. iIntros (tid) "H". eauto. Qed.
+  Global Instance perm_equiv : Equiv perm :=
+    λ ρ1 ρ2, perm_incl ρ1 ρ2 ∧ perm_incl ρ2 ρ1.
 
-  Global Instance perm_incl_refl : Reflexive perm_incl.
-  Proof. iIntros (? tid) "H". eauto. Qed.
+  Class Duplicable (ρ : @perm Σ) :=
+    perm_incl_duplicable : perm_incl ρ (ρ ★ ρ).
 
-  Global Instance perm_incl_trans : Transitive perm_incl.
-  Proof.
-    iIntros (??? H12 H23 tid) "H". iVs (H12 with "H") as "H". by iApply H23.
-  Qed.
+End defs.
 
-  Lemma perm_incl_frame_l ρ ρ1 ρ2 :
-    perm_incl ρ1 ρ2 → perm_incl (ρ ★ ρ1) (ρ ★ ρ2).
-  Proof. iIntros (Hρ tid) "[$?]". by iApply Hρ. Qed.
+Infix "⇒" := perm_incl (at level 95, no associativity) : C_scope.
+Notation "(⇒)" := perm_incl (only parsing) : C_scope.
 
-  Lemma perm_incl_frame_r ρ ρ1 ρ2 :
-    perm_incl ρ1 ρ2 → perm_incl (ρ1 ★ ρ) (ρ2 ★ ρ).
-  Proof. iIntros (Hρ tid) "[?$]". by iApply Hρ. Qed.
+Notation "ρ1 ⇔ ρ2" := (equiv (A:=perm) ρ1%P ρ2%P)
+   (at level 95, no associativity) : C_scope.
+Notation "(⇔)" := (equiv (A:=perm)) (only parsing) : C_scope.
 
-End perm_incl.
-
-Section duplicable.
+Section props.
 
   Context `{heapG Σ, lifetimeG Σ, thread_localG Σ}.
 
-  Class Duplicable (ρ : perm) :=
-    perm_incl_duplicable : perm_incl ρ (ρ ★ ρ).
+  (* Properties *)
+  Global Instance perm_incl_preorder : PreOrder (⇒).
+  Proof.
+    split.
+    - iIntros (? tid) "H". eauto.
+    - iIntros (??? H12 H23 tid) "H". iVs (H12 with "H") as "H". by iApply H23.
+  Qed.
+
+  Global Instance perm_equiv_equiv : Equivalence (⇔).
+  Proof.
+    split.
+    - by split.
+    - by intros x y []; split.
+    - intros x y z [] []. split; by transitivity y.
+  Qed.
+
+  Global Instance perm_incl_proper :
+    Proper ((⇔) ==> (⇔) ==> iff) (⇒).
+  Proof. intros ??[??]??[??]; split; intros ?; by simplify_order. Qed.
+
+  Lemma perm_incl_top ρ : ρ ⇒ ⊤.
+  Proof. iIntros (tid) "H". eauto. Qed.
+
+  Lemma perm_incl_frame_l ρ ρ1 ρ2 : ρ1 ⇒ ρ2 → ρ ★ ρ1 ⇒ ρ ★ ρ2.
+  Proof. iIntros (Hρ tid) "[$?]". by iApply Hρ. Qed.
+
+  Lemma perm_incl_frame_r ρ ρ1 ρ2 :
+    ρ1 ⇒ ρ2 → ρ1 ★ ρ ⇒ ρ2 ★ ρ.
+  Proof. iIntros (Hρ tid) "[?$]". by iApply Hρ. Qed.
+
+  Lemma perm_incl_exists_intro {A} P x : P x ⇒ ∃ x : A, P x.
+  Proof. iIntros (tid) "H!==>". by iExists x. Qed.
+
+  Global Instance perm_sep_assoc : Assoc (⇔) sep.
+  Proof. intros ???; split. by iIntros (tid) "[$[$$]]". by iIntros (tid) "[[$$]$]". Qed.
+
+  Global Instance perm_sep_comm : Comm (⇔) sep.
+  Proof. intros ??; split; by iIntros (tid) "[$$]". Qed.
+
+  Global Instance perm_top_right_id : RightId (⇔) ⊤ sep.
+  Proof. intros ρ; split. by iIntros (tid) "[? _]". by iIntros (tid) "$". Qed.
+
+  Global Instance perm_top_left_id : LeftId (⇔) ⊤ sep.
+  Proof. intros ρ. by rewrite comm right_id. Qed.
+
+  Lemma perm_tok_plus κ q1 q2 :
+    tok κ q1 ★ tok κ q2 ⇔ tok κ (q1 + q2).
+  Proof.
+    rewrite /tok /sep /=; split; intros tid; rewrite -lft_own_op;
+      iIntros "[[$$]H]!==>". by iDestruct "H" as "[$?]". by auto.
+  Qed.
+
+  Lemma perm_lftincl_refl κ : ⊤ ⇒ κ ⊑ κ.
+  Proof. iIntros (tid) "_!==>". iApply lft_incl_refl. Qed.
+
+  Lemma perm_lftincl_trans κ1 κ2 κ3 : κ1 ⊑ κ2 ★ κ2 ⊑ κ3 ⇒ κ1 ⊑ κ3.
+  Proof. iIntros (tid) "[#?#?]!==>". iApply lft_incl_trans. auto. Qed.
+
+  Lemma perm_incl_share v κ ty :
+    v ◁ &uniq{κ} ty ⇒ v ◁ &shr{κ} ty.
+  Proof.
+    iIntros (tid) "Huniq". iDestruct "Huniq" as (l) "[% Hown]".
+    (* FIXME : we nee some tokens here. *)
+    iAssert (∃ q, [κ]{q})%I as "Htok". admit.
+    iDestruct "Htok" as (q) "Htok".
+    iVs (ty.(ty_share) _ lrustN with "Hown Htok") as "[Hown _]".
+    admit. set_solver. iVsIntro. iExists _. iSplit. done. done.
+  Admitted.
 
   Lemma has_type_dup v ty : ty.(ty_dup) → Duplicable (v ◁ ty).
-  Proof. iIntros (Hdup tid) "H!==>". by iApply ty_dup_dup. Qed.
+  Proof. iIntros (Hdup tid) "H". by iApply ty_dup_dup. Qed.
 
   Global Instance lft_incl_dup κ κ' : Duplicable (κ ⊑ κ').
   Proof. iIntros (tid) "#H!==>". by iSplit. Qed.
@@ -53,39 +116,6 @@ Section duplicable.
   Global Instance top_dup : Duplicable ⊤.
   Proof. iIntros (tid) "_!==>". by iSplit. Qed.
 
-End duplicable.
+End props.
 
 Hint Extern 0 (Duplicable (_ ◁ _)) => apply has_type_dup; exact I.
-
-Section perm_equiv.
-
-  Context `{heapG Σ, lifetimeG Σ, thread_localG Σ}.
-
-  Definition perm_equiv ρ1 ρ2 := perm_incl ρ1 ρ2 ∧ perm_incl ρ2 ρ1.
-
-  Global Instance perm_equiv_refl : Reflexive perm_equiv.
-  Proof. by split. Qed.
-
-  Global Instance perm_equiv_trans : Transitive perm_equiv.
-  Proof. intros x y z [] []. split; by transitivity y. Qed.
-
-  Global Instance perm_equiv_sym : Symmetric perm_equiv.
-  Proof. by intros x y []; split. Qed.
-
-  Global Instance perm_incl_proper :
-    Proper (perm_equiv ==> perm_equiv ==> iff) perm_incl.
-  Proof. intros ??[??]??[??]; split; eauto using perm_incl_trans. Qed.
-
-  Global Instance sep_assoc : Assoc perm_equiv Perm.sep.
-  Proof. intros ???; split. by iIntros (tid) "[$[$$]]". by iIntros (tid) "[[$$]$]". Qed.
-
-  Global Instance sep_comm : Comm perm_equiv Perm.sep.
-  Proof. intros ??; split; by iIntros (tid) "[$$]". Qed.
-
-  Global Instance top_right_id : RightId perm_equiv ⊤ Perm.sep.
-  Proof. intros ρ; split. by iIntros (tid) "[? _]". by iIntros (tid) "$". Qed.
-
-  Global Instance top_left_id : LeftId perm_equiv ⊤ Perm.sep.
-  Proof. intros ρ. by rewrite comm right_id. Qed.
-
-End perm_equiv.
